ExistentialRules/ChaseSequence/Termination/BacktrackingOfFacts.lean
@@ -1,8 +1,8 @@
 module
 
-import ExistentialRules.ChaseSequence.Termination.BacktrackingOfFacts.Basic
-import ExistentialRules.ChaseSequence.Termination.BacktrackingOfFacts.PreGroundTerm
-import ExistentialRules.ChaseSequence.Termination.BacktrackingOfFacts.GroundTerm
-import ExistentialRules.ChaseSequence.Termination.BacktrackingOfFacts.PreTrigger
-import ExistentialRules.ChaseSequence.Termination.BacktrackingOfFacts.ChaseBranch
+public import ExistentialRules.ChaseSequence.Termination.BacktrackingOfFacts.Basic
+public import ExistentialRules.ChaseSequence.Termination.BacktrackingOfFacts.PreGroundTerm
+public import ExistentialRules.ChaseSequence.Termination.BacktrackingOfFacts.GroundTerm
+public import ExistentialRules.ChaseSequence.Termination.BacktrackingOfFacts.PreTrigger
+public import ExistentialRules.ChaseSequence.Termination.BacktrackingOfFacts.ChaseBranch
 
